Nova organização

Modal Logic/.Makefile.d
@@ -1,6 +1,9 @@
-ml1_soundness.vo ml1_soundness.glob ml1_soundness.v.beautified ml1_soundness.required_vo: ml1_soundness.v 
-ml1_soundness.vio: ml1_soundness.v 
-ml1_soundness.vos ml1_soundness.vok ml1_soundness.required_vos: ml1_soundness.v 
+ml0_base.vo ml0_base.glob ml0_base.v.beautified ml0_base.required_vo: ml0_base.v 
+ml0_base.vio: ml0_base.v 
+ml0_base.vos ml0_base.vok ml0_base.required_vos: ml0_base.v 
+ml1_soundness.vo ml1_soundness.glob ml1_soundness.v.beautified ml1_soundness.required_vo: ml1_soundness.v ml0_base.vo
+ml1_soundness.vio: ml1_soundness.v ml0_base.vio
+ml1_soundness.vos ml1_soundness.vok ml1_soundness.required_vos: ml1_soundness.v ml0_base.vos
 ml2_completeness.vo ml2_completeness.glob ml2_completeness.v.beautified ml2_completeness.required_vo: ml2_completeness.v ml1_soundness.vo
 ml2_completeness.vio: ml2_completeness.v ml1_soundness.vio
 ml2_completeness.vos ml2_completeness.vok ml2_completeness.required_vos: ml2_completeness.v ml1_soundness.vos
