Modal Logic/ml2_completeness.v
@@ -7,21 +7,21 @@ Module Type mod_complete (B: mod_base) (S: mod_sound B).
 Import B S.
 
 Inductive NNF : Set :=
-| NPos : VarProp -> NNF
-| NNeg : VarProp -> NNF
+| NPos : VProp -> NNF
+| NNeg : VProp -> NNF
 | NBot : NNF
 | NTop : NNF
 | NConj : NNF -> NNF -> NNF
 | NDisj : NNF -> NNF -> NNF.
 
-Fixpoint MakeNNF (A : FormProp) : NNF := match A with
+Fixpoint MakeNNF (A : FProp) : NNF := match A with
 | # P => NPos P
 | ⊥ => NBot
 | B ∨ C => NDisj (MakeNNF B) (MakeNNF C)
 | B ∧ C => NConj (MakeNNF B) (MakeNNF C)
 | B → C => NDisj (MakeNNFN B) (MakeNNF C)
 end
-with MakeNNFN (A : FormProp) : NNF := match A with
+with MakeNNFN (A : FProp) : NNF := match A with
 | # P => NNeg P
 | ⊥ => NTop
 | B ∨ C => NConj (MakeNNFN B) (MakeNNFN C)
@@ -29,18 +29,18 @@ with MakeNNFN (A : FormProp) : NNF := match A with
 | B → C => NConj (MakeNNF B) (MakeNNFN C)
 end.
 
-Fixpoint NNFtoFormProp (A : NNF) : FormProp := match A with
+Fixpoint NNFtoFProp (A : NNF) : FProp := match A with
 | NPos P => # P
 | NNeg P => ¬ # P
 | NBot => ⊥
 | NTop => ¬ ⊥
-| NConj B C => NNFtoFormProp B ∧ NNFtoFormProp C
-| NDisj B C => NNFtoFormProp B ∨ NNFtoFormProp C
+| NConj B C => NNFtoFProp B ∧ NNFtoFProp C
+| NDisj B C => NNFtoFProp B ∨ NNFtoFProp C
 end.
 
 Inductive Literal :=
-| LPos : VarProp -> Literal
-| LNeg : VarProp -> Literal
+| LPos : VProp -> Literal
+| LNeg : VProp -> Literal
 | LBot : Literal
 | LTop : Literal.
 
@@ -51,7 +51,7 @@ Fixpoint Bar P := match P with
 | LTop => LBot
 end.
 
-Fixpoint LiteraltoFormProp (P : Literal) : FormProp :=
+Fixpoint LiteraltoFProp (P : Literal) : FProp :=
 match P with
 | LPos Q => # Q
 | LNeg Q => ¬ # Q
@@ -59,18 +59,13 @@ match P with
 | LTop => ¬ ⊥
 end.
 
-Fixpoint map_fold_right (A B :Type) (f : B -> A) (g : A -> A -> A) a l := match l with
-| nil => a
-| b :: l2 => g (f b) (map_fold_right f g a l2)
-end.
-
 Definition Clause := list Literal.
 
-Definition ClausetoFormProp := map_fold_right LiteraltoFormProp Disj ⊥.
+Definition ClausetoFProp := map_fold_right LiteraltoFProp Disj ⊥.
 
 Definition CNF := list Clause.
 
-Definition CNFtoFormProp := map_fold_right ClausetoFormProp Conj ⊤.
+Definition CNFtoFProp := map_fold_right ClausetoFProp Conj ⊤.
 
 Definition AddClause (l : Clause) (ll : CNF) : CNF := map (fun l2 => l ++ l2) ll.
 
@@ -90,44 +85,44 @@ Definition Valid_Clause (l : Clause) := In LTop l \/ exists A, (In (LPos A) l /\
 Definition Valid_CNF ll := forall l, In l ll -> Valid_Clause l.
 
 Lemma Literal_eqdec : forall x y : Literal, {x = y} + {x <> y}.
-intros; destruct x; destruct y; try (right; discriminate); try (left; reflexivity); destruct (VarSeq v v0);  (left; f_equal; assumption)||(right; intro HH; injection HH; contradiction).
+intros; destruct x; destruct y; try (right; discriminate); try (left; reflexivity); destruct (VarSeq_dec v v0);  (left; f_equal; assumption)||(right; intro HH; injection HH; contradiction).
 Qed.
 
-Lemma NNF_equiv_valid : forall v A, TrueQ v (NNFtoFormProp (MakeNNF  A)) = TrueQ v A /\ TrueQ v (NNFtoFormProp (MakeNNFN A)) = TrueQ v ¬ A.
+Lemma NNF_equiv_valid : forall v A, TrueQ v (NNFtoFProp (MakeNNF  A)) = TrueQ v A /\ TrueQ v (NNFtoFProp (MakeNNFN A)) = TrueQ v ¬ A.
 intros v A; induction A; try destruct IHA; try destruct IHA1; try destruct IHA2; split; simpl in *; try trivial; try rewrite H; try rewrite H0; try rewrite H1; try rewrite H2; try trivial; repeat rewrite orb_false_r; repeat rewrite orb_false_l; try rewrite negb_andb; try rewrite negb_orb; try rewrite negb_involutive; reflexivity.
 Qed.
 
-Lemma CNF_and_valid : forall v ll1 ll2, TrueQ v (CNFtoFormProp (ll1 ++ ll2)) = TrueQ v (CNFtoFormProp ll1) && TrueQ v (CNFtoFormProp ll2).
+Lemma CNF_and_valid : forall v ll1 ll2, TrueQ v (CNFtoFProp (ll1 ++ ll2)) = TrueQ v (CNFtoFProp ll1) && TrueQ v (CNFtoFProp ll2).
 intros; induction ll1; simpl.
 reflexivity.
-unfold CNFtoFormProp in IHll1 at 1; rewrite IHll1.
+unfold CNFtoFProp in IHll1 at 1; rewrite IHll1.
 apply andb_assoc.
 Qed.
 
-Lemma CNF_or_clause_valid : forall v l1 l2, TrueQ v (ClausetoFormProp (l1 ++ l2)) = TrueQ v (ClausetoFormProp l1) || TrueQ v (ClausetoFormProp l2).
+Lemma CNF_or_clause_valid : forall v l1 l2, TrueQ v (ClausetoFProp (l1 ++ l2)) = TrueQ v (ClausetoFProp l1) || TrueQ v (ClausetoFProp l2).
 intros; induction l1; simpl.
 reflexivity.
-unfold ClausetoFormProp in IHl1 at 1; rewrite IHl1.
+unfold ClausetoFProp in IHl1 at 1; rewrite IHl1.
 apply orb_assoc.
 Qed.
 
-Lemma CNF_add_clause_valid : forall v l ll, TrueQ v (CNFtoFormProp (AddClause l ll)) = TrueQ v (ClausetoFormProp l) || TrueQ v (CNFtoFormProp ll).
+Lemma CNF_add_clause_valid : forall v l ll, TrueQ v (CNFtoFProp (AddClause l ll)) = TrueQ v (ClausetoFProp l) || TrueQ v (CNFtoFProp ll).
 intros; induction ll; simpl.
 rewrite orb_true_r; reflexivity.
-unfold CNFtoFormProp in IHll at 1; rewrite IHll.
+unfold CNFtoFProp in IHll at 1; rewrite IHll.
 rewrite CNF_or_clause_valid.
 rewrite orb_andb_distrib_r.
 reflexivity.
 Qed.
 
-Lemma CNF_or_valid : forall v ll1 ll2, TrueQ v (CNFtoFormProp (Disjunct ll1 ll2)) = TrueQ v (CNFtoFormProp ll1) || TrueQ v (CNFtoFormProp ll2).
+Lemma CNF_or_valid : forall v ll1 ll2, TrueQ v (CNFtoFProp (Disjunct ll1 ll2)) = TrueQ v (CNFtoFProp ll1) || TrueQ v (CNFtoFProp ll2).
 intros; induction ll1; simpl.
 reflexivity.
 rewrite CNF_and_valid; rewrite IHll1; rewrite CNF_add_clause_valid.
 rewrite orb_andb_distrib_l; reflexivity.
 Qed.
 
-Theorem CNF_equiv_valid : forall v A, TrueQ v (CNFtoFormProp (MakeCNF A)) = TrueQ v (NNFtoFormProp A).
+Theorem CNF_equiv_valid : forall v A, TrueQ v (CNFtoFProp (MakeCNF A)) = TrueQ v (NNFtoFProp A).
 intros; induction A; simpl; try reflexivity; try (destruct (v v0); simpl; reflexivity; fail); [rewrite CNF_and_valid|rewrite CNF_or_valid]; rewrite IHA1; rewrite IHA2; reflexivity.
 Qed.
 
@@ -135,15 +130,15 @@ Definition Countervaluation l P := if (in_dec Literal_eqdec (LNeg P) l) then tru
 
 Definition Validates v Δ := exists A, In A Δ /\ Is_true (TrueQ v A).
 
-Lemma TrueQ_impl_Validates : forall v m, Is_true (TrueQ v (ClausetoFormProp m)) -> Validates v (map LiteraltoFormProp m).
+Lemma TrueQ_impl_Validates : forall v m, Is_true (TrueQ v (ClausetoFProp m)) -> Validates v (map LiteraltoFProp m).
 intros; induction m.
 contradiction.
-simpl in H; case_bool v (LiteraltoFormProp a).
-exists (LiteraltoFormProp a); split; [in_solve|rewrite H0; trivial].
+simpl in H; case_bool v (LiteraltoFProp a).
+exists (LiteraltoFProp a); split; [in_solve|rewrite H0; trivial].
 destruct (IHm H) as (?&?&?); exists x; split; [in_solve|assumption].
 Qed.
 
-Lemma Validated_valid : forall l, Validates (Countervaluation l) (map LiteraltoFormProp l) -> Valid_Clause l.
+Lemma Validated_valid : forall l, Validates (Countervaluation l) (map LiteraltoFProp l) -> Valid_Clause l.
 intros l (A&H&K).
 apply in_map_iff in H as (p&?&H); subst; destruct p; unfold Countervaluation in K; simpl in K.
 destruct (in_dec Literal_eqdec (LNeg v) l).
@@ -154,13 +149,13 @@ contradiction.
 left; assumption.
 Qed.
 
-Theorem Clause_valid : forall l, Valid (ClausetoFormProp l) -> Valid_Clause l.
+Theorem Clause_valid : forall l, Valid (ClausetoFProp l) -> Valid_Clause l.
 intros; apply Validated_valid; apply TrueQ_impl_Validates; apply H; intros ? Q; destruct Q.
 Qed.
 
-Theorem CNF_valid : forall ll, Valid (CNFtoFormProp ll) -> Valid_CNF ll.
+Theorem CNF_valid : forall ll, Valid (CNFtoFProp ll) -> Valid_CNF ll.
 induction ll; intros ? ? H0; destruct H0; subst.
-apply Clause_valid; intros v K; remember (H v K) as i eqn:x; clear x; simpl in i; case_bool v (ClausetoFormProp l).
+apply Clause_valid; intros v K; remember (H v K) as i eqn:x; clear x; simpl in i; case_bool v (ClausetoFProp l).
 apply IHll.
 intros v K.
 remember (H v K).
@@ -172,19 +167,19 @@ eapply H; assumption.
 assumption.
 Qed.
 
-Lemma Clause_provable_3 : forall a l1 l2 Γ, In (LiteraltoFormProp a) Γ -> Γ ⊢ ClausetoFormProp (l1 ++ a :: l2).
+Lemma Clause_provable_3 : forall a l1 l2 Γ, In (LiteraltoFProp a) Γ -> Γ ⊢ ClausetoFProp (l1 ++ a :: l2).
 intros; induction l1.
 apply OrI1; is_ass.
 apply OrI2; assumption.
 Qed.
 
-Lemma Clause_provable_2 : forall a l1 l2 l3, Provable (ClausetoFormProp (l1 ++ (Bar a) :: l2 ++ a :: l3)).
+Lemma Clause_provable_2 : forall a l1 l2 l3, Provable (ClausetoFProp (l1 ++ (Bar a) :: l2 ++ a :: l3)).
 intros; induction l1.
 apply BotC; mp; [is_ass|destruct a; simpl; apply OrI1]; try (apply ImpI; mp; [is_ass|apply OrI2; apply Clause_provable_3; in_solve]); (apply BotC; mp; [constructor; constructor 2; in_solve|apply OrI2; apply Clause_provable_3; in_solve]).
 apply OrI2; assumption.
 Qed.
 
-Theorem Clause_provable : forall l, Valid_Clause l -> Provable (ClausetoFormProp l).
+Theorem Clause_provable : forall l, Valid_Clause l -> Provable (ClausetoFProp l).
 intros ? [?|(?&?&?)]; apply in_split in H as (?&?&?); subst.
 induction x; simpl.
 apply OrI1; simpl; apply ImpI; is_ass.
@@ -197,8 +192,8 @@ apply in_split in H0 as (?&?&?); subst.
 apply (Clause_provable_2 (LNeg x)).
 Qed.
 
-Theorem CNF_provable : forall ll, Valid_CNF ll -> Provable (CNFtoFormProp ll).
-intros; induction ll; unfold CNFtoFormProp; simpl.
+Theorem CNF_provable : forall ll, Valid_CNF ll -> Provable (CNFtoFProp ll).
+intros; induction ll; unfold CNFtoFProp; simpl.
 apply ImpI;is_ass.
 eapply AndI.
 apply Clause_provable; apply H; constructor; reflexivity.
@@ -210,14 +205,14 @@ intros; prov_impl_in H; prov_impl_in H0.
 apply AndI; [apply K;eapply AndE1|apply K0; eapply AndE2]; is_ass.
 Qed.
 
-Lemma CNF_and_prov : forall ll1 ll2, Provable (CNFtoFormProp (ll1 ++ ll2) → CNFtoFormProp ll1 ∧ CNFtoFormProp ll2).
+Lemma CNF_and_prov : forall ll1 ll2, Provable (CNFtoFProp (ll1 ++ ll2) → CNFtoFProp ll1 ∧ CNFtoFProp ll2).
 intros; induction ll1; simpl.
-unfold CNFtoFormProp at 2; unfold ClausetoFormProp; simpl.
+unfold CNFtoFProp at 2; unfold ClausetoFProp; simpl.
 apply ImpI; apply AndI.
 unfold Top; unfold Neg; apply ImpI; is_ass.
 is_ass.
 prov_impl_in IHll1; apply ImpI; apply AndI.
-unfold CNFtoFormProp; simpl; apply AndI.
+unfold CNFtoFProp; simpl; apply AndI.
 eapply AndE1; is_ass.
 eapply AndE1; apply K.
 eapply AndE2; is_ass.
@@ -232,56 +227,56 @@ apply OrI1; apply K; is_ass.
 apply OrI2; apply K0; is_ass.
 Qed.
 
-Lemma CNF_or_clause_prov : forall l1 l2, Provable (ClausetoFormProp (l1 ++ l2) → ClausetoFormProp l1 ∨ ClausetoFormProp l2).
-intros; induction l1; simpl; unfold ClausetoFormProp; simpl.
+Lemma CNF_or_clause_prov : forall l1 l2, Provable (ClausetoFProp (l1 ++ l2) → ClausetoFProp l1 ∨ ClausetoFProp l2).
+intros; induction l1; simpl; unfold ClausetoFProp; simpl.
 apply ImpI; eapply OrI2; is_ass.
 prov_impl_in IHl1.
 apply ImpI.
 eapply OrE.
 is_ass.
 do 2 eapply OrI1; is_ass.
-apply OrE with (ClausetoFormProp l1) (ClausetoFormProp l2).
+apply OrE with (ClausetoFProp l1) (ClausetoFProp l2).
 apply K; is_ass.
 apply OrI1; apply OrI2; is_ass.
 apply OrI2; is_ass.
 Qed.
 
-Lemma CNF_add_clause_prov : forall l ll, Provable (CNFtoFormProp (AddClause l ll) → ClausetoFormProp l ∨ CNFtoFormProp ll).
-intros; induction ll; simpl; unfold CNFtoFormProp; simpl.
+Lemma CNF_add_clause_prov : forall l ll, Provable (CNFtoFProp (AddClause l ll) → ClausetoFProp l ∨ CNFtoFProp ll).
+intros; induction ll; simpl; unfold CNFtoFProp; simpl.
 apply ImpI; eapply OrI2; is_ass.
-prov_impl_in IHll; apply ImpI; apply OrE with (ClausetoFormProp l) (ClausetoFormProp a).
+prov_impl_in IHll; apply ImpI; apply OrE with (ClausetoFProp l) (ClausetoFProp a).
 eapply prov_impl.
 apply CNF_or_clause_prov.
 eapply AndE1; is_ass.
 apply OrI1; is_ass.
-apply OrE with (ClausetoFormProp l) (CNFtoFormProp ll).
+apply OrE with (ClausetoFProp l) (CNFtoFProp ll).
 apply K; eapply AndE2; is_ass.
 apply OrI1; is_ass.
 apply OrI2; apply AndI; is_ass.
 Qed.
 
-Lemma CNF_or_prov : forall ll1 ll2, Provable (CNFtoFormProp (Disjunct ll1 ll2) → CNFtoFormProp ll1 ∨ CNFtoFormProp ll2).
-intros; induction ll1; simpl; unfold CNFtoFormProp; simpl.
+Lemma CNF_or_prov : forall ll1 ll2, Provable (CNFtoFProp (Disjunct ll1 ll2) → CNFtoFProp ll1 ∨ CNFtoFProp ll2).
+intros; induction ll1; simpl; unfold CNFtoFProp; simpl.
 apply ImpI; eapply OrI1; is_ass.
-prov_impl_in IHll1; apply ImpI; apply OrE with (ClausetoFormProp a) (CNFtoFormProp ll2).
+prov_impl_in IHll1; apply ImpI; apply OrE with (ClausetoFProp a) (CNFtoFProp ll2).
 eapply prov_impl; [apply CNF_add_clause_prov|].
 eapply AndE1; eapply prov_impl; [apply CNF_and_prov|is_ass].
-apply OrE with (CNFtoFormProp ll1) (CNFtoFormProp ll2).
+apply OrE with (CNFtoFProp ll1) (CNFtoFProp ll2).
 apply K; eapply AndE2; eapply prov_impl; [apply CNF_and_prov|is_ass].
 apply OrI1; apply AndI; is_ass.
 apply OrI2; is_ass.
 apply OrI2; is_ass.
 Qed.
 
-Theorem CNF_impl_prov : forall A, Provable (CNFtoFormProp (MakeCNF A) → NNFtoFormProp A).
-induction A; simpl; try (unfold CNFtoFormProp; unfold ClausetoFormProp; simpl; apply Impl; eapply OrE; [eapply AndE1; is_ass|is_ass|apply BotC; is_ass]; fail).
+Theorem CNF_impl_prov : forall A, Provable (CNFtoFProp (MakeCNF A) → NNFtoFProp A).
+induction A; simpl; try (unfold CNFtoFProp; unfold ClausetoFProp; simpl; apply Impl; eapply OrE; [eapply AndE1; is_ass|is_ass|apply BotC; is_ass]; fail).
 apply ImpI; apply AndI; (eapply prov_impl; [eassumption|]); [eapply AndE1|eapply AndE2]; (eapply prov_impl; [apply CNF_and_prov|is_ass]).
 apply ImpI; eapply prov_impl.
 apply ImpI; eapply prov_or; try eassumption; in_solve.
 eapply prov_impl; [apply CNF_or_prov|is_ass].
 Qed.
 
-Lemma NNF_impl_prov : forall A, Provable (NNFtoFormProp (MakeNNF  A) →  A) /\ Provable (NNFtoFormProp (MakeNNFN A) → ¬A).
+Lemma NNF_impl_prov : forall A, Provable (NNFtoFProp (MakeNNF  A) →  A) /\ Provable (NNFtoFProp (MakeNNFN A) → ¬A).
 induction A; simpl; split; try destruct IHA; try destruct IHA1; try destruct IHA2; apply ImpI; try (is_ass; fail).
 eapply prov_and; try eassumption; in_solve.
 apply ImpI.
