Modal Logic/ml0_base.v
@@ -1,0 +1,20 @@
+(* Preâmbulo *)
+Set Implicit Arguments.
+Require Export Bool.
+Require Export List.
+Import ListNotations.
+(* Módulo Base *)
+Module Type mod_base.
+(* Meu escopo *)
+Declare Scope My_scope.
+Open Scope My_scope.
+(* Conjunto das Variáveis Proposicionais *)
+Parameter VProp : Set.
+(* Igualdade é decidível em VarProp *)
+Parameter VarSeq_dec : forall x y: VProp, {x = y} + {x <> y}.
+(* Função usada em  ml1_soundness *)
+Fixpoint map_fold_right (A B :Type) (f : B -> A) (g : A -> A -> A) a l := match l with
+| nil => a
+| b :: l2 => g (f b) (map_fold_right f g a l2)
+end.
+End mod_base.
